Arithmetization/ISigmaOne/Metamath/Term.lean
@@ -7,17 +7,17 @@ namespace LO.Arith
 
 open FirstOrder FirstOrder.Arith
 
-variable {M : Type*} [Zero M] [One M] [Add M] [Mul M] [LT M] [M ⊧ₘ* 𝐈𝚺₁]
+variable {V : Type*} [Zero V] [One V] [Add V] [Mul V] [LT V] [V ⊧ₘ* 𝐈𝚺₁]
 
-variable {L : Arith.Language M} {pL : LDef} [Arith.Language.Defined L pL]
+variable {L : Arith.Language V} {pL : LDef} [Arith.Language.Defined L pL]
 
 section term
 
-def qqBvar (z : M) : M := ⟪0, z⟫ + 1
+def qqBvar (z : V) : V := ⟪0, z⟫ + 1
 
-def qqFvar (x : M) : M := ⟪1, x⟫ + 1
+def qqFvar (x : V) : V := ⟪1, x⟫ + 1
 
-def qqFunc (k f v : M) : M := ⟪2, k, f, v⟫ + 1
+def qqFunc (k f v : V) : V := ⟪2, k, f, v⟫ + 1
 
 scoped prefix:max "^#" => qqBvar
 
@@ -25,51 +25,51 @@ scoped prefix:max "^&" => qqFvar
 
 scoped prefix:max "^func " => qqFunc
 
-@[simp] lemma var_lt_qqBvar (z : M) : z < ^#z := lt_succ_iff_le.mpr <| le_pair_right 0 z
+@[simp] lemma var_lt_qqBvar (z : V) : z < ^#z := lt_succ_iff_le.mpr <| le_pair_right 0 z
 
-@[simp] lemma var_lt_qqFvar (x : M) : x < ^&x := lt_succ_iff_le.mpr <| le_pair_right 1 x
+@[simp] lemma var_lt_qqFvar (x : V) : x < ^&x := lt_succ_iff_le.mpr <| le_pair_right 1 x
 
-@[simp] lemma arity_lt_qqFunc (k f v : M) : k < ^func k f v :=
+@[simp] lemma arity_lt_qqFunc (k f v : V) : k < ^func k f v :=
   le_iff_lt_succ.mp <| le_trans (le_pair_right 2 k) <| pair_le_pair_right 2 <| le_pair_left k ⟪f, v⟫
 
-@[simp] lemma func_lt_qqFunc (k f v : M) : f < ^func k f v :=
+@[simp] lemma func_lt_qqFunc (k f v : V) : f < ^func k f v :=
   le_iff_lt_succ.mp <| le_trans (le_pair_left f v) <| le_trans (le_pair_right k ⟪f, v⟫) <| le_pair_right 2 ⟪k, ⟪f, v⟫⟫
 
-@[simp] lemma terms_lt_qqFunc (k f v : M) : v < ^func k f v :=
+@[simp] lemma terms_lt_qqFunc (k f v : V) : v < ^func k f v :=
   le_iff_lt_succ.mp <| le_trans (le_pair_right f v) <| le_trans (le_pair_right k ⟪f, v⟫) <| le_pair_right 2 ⟪k, ⟪f, v⟫⟫
 
-lemma lt_qqFunc_of_mem {i b k f v : M} (hi : ⟪i, b⟫ ∈ v) : b < ^func k f v :=
+lemma lt_qqFunc_of_mem {i b k f v : V} (hi : ⟪i, b⟫ ∈ v) : b < ^func k f v :=
   _root_.lt_trans (lt_of_mem_rng hi) (terms_lt_qqFunc k f v)
 
-@[simp] lemma qqBvar_inj {z z' : M} : ^#z = ^#z' ↔ z = z' := by simp [qqBvar]
+@[simp] lemma qqBvar_inj {z z' : V} : ^#z = ^#z' ↔ z = z' := by simp [qqBvar]
 
-@[simp] lemma qqFvar_inj {x x' : M} : ^&x = ^&x' ↔ x = x' := by simp [qqFvar]
+@[simp] lemma qqFvar_inj {x x' : V} : ^&x = ^&x' ↔ x = x' := by simp [qqFvar]
 
-@[simp] lemma qqFunc_inj {k f v k' f' v' : M} : ^func k f v = ^func k' f' v' ↔ k = k' ∧ f = f' ∧ v = v' := by simp [qqFunc]
+@[simp] lemma qqFunc_inj {k f v k' f' v' : V} : ^func k f v = ^func k' f' v' ↔ k = k' ∧ f = f' ∧ v = v' := by simp [qqFunc]
 
 def _root_.LO.FirstOrder.Arith.qqBvarDef : 𝚺₀-Semisentence 2 := .mkSigma “t z | ∃ t' < t, !pairDef t' 0 z ∧ t = t' + 1” (by simp)
 
-lemma qqBvar_defined : 𝚺₀-Function₁ (qqBvar : M → M) via qqBvarDef := by
+lemma qqBvar_defined : 𝚺₀-Function₁ (qqBvar : V → V) via qqBvarDef := by
   intro v; simp [qqBvarDef]
   constructor
   · intro h; exact ⟨⟪0, v 1⟫, by simp [qqBvar, h], rfl, h⟩
   · rintro ⟨x, _, rfl, h⟩; exact h
 
 @[simp] lemma eval_qqBvarDef (v) :
-    Semiformula.Evalbm M v qqBvarDef.val ↔ v 0 = ^#(v 1) := qqBvar_defined.df.iff v
+    Semiformula.Evalbm V v qqBvarDef.val ↔ v 0 = ^#(v 1) := qqBvar_defined.df.iff v
 
 def _root_.LO.FirstOrder.Arith.qqFvarDef : 𝚺₀-Semisentence 2 := .mkSigma “t x | ∃ t' < t, !pairDef t' 1 x ∧ t = t' + 1” (by simp)
 
-lemma qqFvar_defined : 𝚺₀-Function₁ (qqFvar : M → M) via qqFvarDef := by
+lemma qqFvar_defined : 𝚺₀-Function₁ (qqFvar : V → V) via qqFvarDef := by
   intro v; simp [qqFvarDef]
   constructor
   · intro h; exact ⟨⟪1, v 1⟫, by simp [qqFvar, h], rfl, h⟩
   · rintro ⟨x, _, rfl, h⟩; exact h
 
 @[simp] lemma eval_qqFvarDef (v) :
-    Semiformula.Evalbm M v qqFvarDef.val ↔ v 0 = ^&(v 1) := qqFvar_defined.df.iff v
+    Semiformula.Evalbm V v qqFvarDef.val ↔ v 0 = ^&(v 1) := qqFvar_defined.df.iff v
 
-private lemma qqFunc_graph {x k f v : M} :
+private lemma qqFunc_graph {x k f v : V} :
     x = ^func k f v ↔ ∃ fv < x, fv = ⟪f, v⟫ ∧ ∃ kfv < x, kfv = ⟪k, fv⟫ ∧ ∃ x' < x, x' = ⟪2, kfv⟫ ∧ x = x' + 1 :=
   ⟨by rintro rfl
       exact ⟨⟪f, v⟫, lt_succ_iff_le.mpr <| le_trans (le_pair_right _ _) (le_pair_right _ _), rfl,
@@ -80,20 +80,20 @@ private lemma qqFunc_graph {x k f v : M} :
 def _root_.LO.FirstOrder.Arith.qqFuncDef : 𝚺₀-Semisentence 4 := .mkSigma
   “x k f v | ∃ fv < x, !pairDef fv f v ∧ ∃ kfv < x, !pairDef kfv k fv ∧ ∃ x' < x, !pairDef x' 2 kfv ∧ x = x' + 1” (by simp)
 
-lemma qqFunc_defined : 𝚺₀-Function₃ (qqFunc : M → M → M → M) via qqFuncDef := by
+lemma qqFunc_defined : 𝚺₀-Function₃ (qqFunc : V → V → V → V) via qqFuncDef := by
   intro v; simp [qqFuncDef, qqFunc_graph]
 
 @[simp] lemma eval_qqFuncDef (v) :
-    Semiformula.Evalbm M v qqFuncDef.val ↔ v 0 = ^func (v 1) (v 2) (v 3) := qqFunc_defined.df.iff v
+    Semiformula.Evalbm V v qqFuncDef.val ↔ v 0 = ^func (v 1) (v 2) (v 3) := qqFunc_defined.df.iff v
 
 namespace FormalizedTerm
 
 variable (L)
 
-def Phi (n : M) (C : Set M) (t : M) : Prop :=
-  (∃ z < n, t = ^#z) ∨ (∃ x, t = ^&x) ∨ (∃ k f v : M, L.Func k f ∧ Seq v ∧ k = lh v ∧ (∀ i u, ⟪i, u⟫ ∈ v → u ∈ C) ∧ t = ^func k f v)
+def Phi (n : V) (C : Set V) (t : V) : Prop :=
+  (∃ z < n, t = ^#z) ∨ (∃ x, t = ^&x) ∨ (∃ k f v : V, L.Func k f ∧ Seq v ∧ k = lh v ∧ (∀ i u, ⟪i, u⟫ ∈ v → u ∈ C) ∧ t = ^func k f v)
 
-private lemma phi_iff (n : M) (C : M) (t : M) :
+private lemma phi_iff (n : V) (C : V) (t : V) :
     Phi L n {x | x ∈ C} t ↔
     (∃ z < n, t = ^#z) ∨
     (∃ x < t, t = ^&x) ∨
@@ -120,7 +120,7 @@ def formula (pL : LDef) : Fixpoint.Blueprint 1 := ⟨.ofZero (.mkSigma
     (∃ k < t, ∃ f < t, ∃ v < t, !pL.func k f ∧ :Seq v ∧ !lhDef k v ∧ (∀ i < v, ∀ u < v, i ~[v] u → u ∈ C) ∧ !qqFuncDef t k f v)”
   (by simp)) _⟩
 
-def construction : Fixpoint.Construction M (formula pL) where
+def construction : Fixpoint.Construction V (formula pL) where
   Φ := fun n ↦ Phi L (n 0)
   defined := .of_zero <| by intro v; simp [phi_iff, Language.Defined.eval_func (L := L) (pL := pL)]
   monotone := by
@@ -129,7 +129,7 @@ def construction : Fixpoint.Construction M (formula pL) where
     · exact Or.inr <| Or.inl h
     · exact Or.inr <| Or.inr ⟨k, f, v, hkf, Sv, hk, fun i u hi ↦ hC (h i u hi), rfl⟩
 
-instance : (construction L).StrongFinite M where
+instance : (construction L).StrongFinite V where
   strong_finite := by
     rintro C v x (h | h | ⟨k, f, v, hkf, Sv, hk, h, rfl⟩)
     · exact Or.inl h
@@ -143,7 +143,7 @@ open FormalizedTerm
 
 variable (L)
 
-def Language.IsSemiterm (n : M) : M → Prop := (construction L).Fixpoint ![n]
+def Language.IsSemiterm (n : V) : V → Prop := (construction L).Fixpoint ![n]
 
 def _root_.LO.FirstOrder.Arith.LDef.isSemitermDef (pL : LDef) : 𝚫₁-Semisentence 2 := (formula pL).fixpointDefΔ₁.rew (Rew.substs ![#1, #0])
 
@@ -152,81 +152,26 @@ lemma isSemiterm_defined : 𝚫₁-Relation L.IsSemiterm via pL.isSemitermDef :=
    by intro v; simp [LDef.isSemitermDef, (construction L).eval_fixpointDefΔ₁]; rfl⟩
 
 @[simp] lemma eval_isSemitermDef (v) :
-    Semiformula.Evalbm M v pL.isSemitermDef.val ↔ L.IsSemiterm (v 0) (v 1) := (isSemiterm_defined L).df.iff v
+    Semiformula.Evalbm V v pL.isSemitermDef.val ↔ L.IsSemiterm (v 0) (v 1) := (isSemiterm_defined L).df.iff v
 
 instance isSemitermDef_definable : 𝚫₁-Relation (L.IsSemiterm) := Defined.to_definable _ (isSemiterm_defined L)
 
 @[simp, definability] instance isSemitermDef_definable' (Γ) : (Γ, m + 1)-Relation (L.IsSemiterm) :=
   .of_deltaOne (isSemitermDef_definable L) _ _
 
-variable {L}
-
-variable {n : M}
-
-local prefix:80 "𝐓ⁿ " => L.IsSemiterm n
-
-lemma Language.IsSemiterm.case_iff {t : M} :
-    𝐓ⁿ t ↔
-    (∃ z < n, t = ^#z) ∨
-    (∃ x, t = ^&x) ∨
-    (∃ k f v : M, L.Func k f ∧ Seq v ∧ k = lh v ∧ (∀ i u, ⟪i, u⟫ ∈ v → 𝐓ⁿ u) ∧ t = ^func k f v) :=
-  (construction L).case
-
-alias ⟨Language.IsSemiterm.case, Language.IsSemiterm.mk⟩ := Language.IsSemiterm.case_iff
-
-@[simp] lemma IsSemiterm.bvar {z : M} : 𝐓ⁿ ^#z ↔ z < n :=
-  ⟨by intro h
-      rcases h.case with (⟨z', hz, hzz'⟩ | ⟨x, h⟩ | ⟨k, f, v, _, _, _, _, h⟩)
-      · rcases (show z = z' from by simpa using hzz'); exact hz
-      · simp [qqBvar, qqFvar] at h
-      · simp [qqBvar, qqFunc] at h,
-    fun hz ↦ Language.IsSemiterm.mk (Or.inl ⟨z, hz, rfl⟩)⟩
-
-@[simp] lemma IsSemiterm.fvar (x : M) : 𝐓ⁿ ^&x := Language.IsSemiterm.mk (Or.inr <| Or.inl ⟨x, rfl⟩)
-
-lemma IsSemiterm.func {k f v : M} (hkf : L.Func k f) (Sv : Seq v) (hk : k = lh v)
-    (h : ∀ i u, ⟪i, u⟫ ∈ v → 𝐓ⁿ u) :
-    𝐓ⁿ (^func k f v) := Language.IsSemiterm.mk (Or.inr <| Or.inr ⟨k, f, v, hkf, Sv, hk, h, rfl⟩)
-
-lemma IsSemiterm.func_iff {k f v : M} :
-    𝐓ⁿ (^func k f v) ↔ L.Func k f ∧ Seq v ∧ k = lh v ∧ ∀ i u, ⟪i, u⟫ ∈ v → 𝐓ⁿ u :=
-  ⟨by intro h
-      rcases h.case with (⟨_, _, h⟩ | ⟨x, h⟩ | ⟨k', f', v', hkf, Sv, hk, hv, h⟩)
-      · simp [qqFunc, qqBvar] at h
-      · simp [qqFunc, qqFvar] at h
-      · rcases (show k = k' ∧ f = f' ∧ v = v' by simpa [qqFunc] using h) with ⟨rfl, rfl, rfl⟩
-        exact ⟨hkf, Sv, hk, hv⟩,
-   by rintro ⟨hkf, Sv, hk, hv⟩; exact IsSemiterm.func hkf Sv hk hv⟩
-
-lemma IsSemiterm.induction (Γ) {P : M → Prop} (hP : (Γ, 1)-Predicate P)
-    (hbvar : ∀ z < n, P (^#z)) (hfvar : ∀ x, P (^&x))
-    (hfunc : ∀ k f v, L.Func k f → Seq v → k = lh v → (∀ i u, ⟪i, u⟫ ∈ v → 𝐓ⁿ u ∧ P u) → P (^func k f v)) :
-    ∀ t, 𝐓ⁿ t → P t :=
-  (construction L).induction (v := ![n]) hP (by
-    rintro C hC x (⟨z, hz, rfl⟩ | ⟨x, rfl⟩ | ⟨k, f, v, hkf, Sv, hk, h, rfl⟩)
-    · exact hbvar z hz
-    · exact hfvar x
-    · exact hfunc k f v hkf Sv hk (fun i u hi ↦ hC u (h i u hi)))
-
-end term
-
-section termSubst
-
-variable (L)
-
-def Language.TermSeq (n m w : M) : Prop := Seq w ∧ n = lh w ∧ ∀ i u, ⟪i, u⟫ ∈ w → L.IsSemiterm m u
+def Language.TermSeq (n m w : V) : Prop := Seq w ∧ n = lh w ∧ ∀ i u, ⟪i, u⟫ ∈ w → L.IsSemiterm m u
 
 variable {L}
 
-protected lemma Language.TermSeq.seq {n m w : M} (h : L.TermSeq n m w) : Seq w := h.1
+protected lemma Language.TermSeq.seq {n m w : V} (h : L.TermSeq n m w) : Seq w := h.1
 
-protected lemma Language.TermSeq.lh {n m w : M} (h : L.TermSeq n m w) : n = lh w := h.2.1
+protected lemma Language.TermSeq.lh {n m w : V} (h : L.TermSeq n m w) : n = lh w := h.2.1
 
-lemma Language.TermSeq.prop {n m w : M} (h : L.TermSeq n m w) : ∀ i u, ⟪i, u⟫ ∈ w → L.IsSemiterm m u := h.2.2
+lemma Language.TermSeq.prop {n m w : V} (h : L.TermSeq n m w) : ∀ i u, ⟪i, u⟫ ∈ w → L.IsSemiterm m u := h.2.2
 
 section
 
-private lemma termSeq_iff (n m w : M) :
+private lemma termSeq_iff (n m w : V) :
     L.TermSeq n m w ↔ Seq w ∧ n = lh w ∧ ∀ i < w, ∀ u < w, ⟪i, u⟫ ∈ w → L.IsSemiterm m u :=
   ⟨fun h ↦ ⟨Language.TermSeq.seq h, Language.TermSeq.lh h, fun i _ u _ hi ↦ Language.TermSeq.prop h i u hi⟩,
    by rintro ⟨Sw, hn, h⟩
@@ -248,7 +193,7 @@ lemma termSeq_defined : 𝚫₁-Relation₃ (L.TermSeq) via pL.termSeqDef :=
    by intro v; simp [LDef.termSeqDef, HSemiformula.val_sigma, eval_isSemitermDef L, termSeq_iff]⟩
 
 @[simp] lemma eval_termSeq (v) :
-    Semiformula.Evalbm M v pL.termSeqDef.val ↔ L.TermSeq (v 0) (v 1) (v 2) := (termSeq_defined L).df.iff v
+    Semiformula.Evalbm V v pL.termSeqDef.val ↔ L.TermSeq (v 0) (v 1) (v 2) := (termSeq_defined L).df.iff v
 
 instance termSeq_definable : 𝚫₁-Relation₃ (L.TermSeq) := Defined.to_definable _ (termSeq_defined L)
 
@@ -257,17 +202,67 @@ instance termSeq_definable : 𝚫₁-Relation₃ (L.TermSeq) := Defined.to_defin
 
 end
 
+variable {n : V}
+
+local prefix:80 "𝐓ⁿ " => L.IsSemiterm n
+
+lemma Language.IsSemiterm.case_iff {t : V} :
+    𝐓ⁿ t ↔
+    (∃ z < n, t = ^#z) ∨
+    (∃ x, t = ^&x) ∨
+    (∃ k f v : V, L.Func k f ∧ L.TermSeq k n v ∧ t = ^func k f v) := by
+  simpa [construction, Phi, TermSeq, and_assoc] using (construction L).case
+
+alias ⟨Language.IsSemiterm.case, Language.IsSemiterm.mk⟩ := Language.IsSemiterm.case_iff
+
+@[simp] lemma IsSemiterm.bvar {z : V} : 𝐓ⁿ ^#z ↔ z < n :=
+  ⟨by intro h
+      rcases h.case with (⟨z', hz, hzz'⟩ | ⟨x, h⟩ | ⟨k, f, v, _, _, h⟩)
+      · rcases (show z = z' from by simpa using hzz'); exact hz
+      · simp [qqBvar, qqFvar] at h
+      · simp [qqBvar, qqFunc] at h,
+    fun hz ↦ Language.IsSemiterm.mk (Or.inl ⟨z, hz, rfl⟩)⟩
+
+@[simp] lemma IsSemiterm.fvar (x : V) : 𝐓ⁿ ^&x := Language.IsSemiterm.mk (Or.inr <| Or.inl ⟨x, rfl⟩)
+
+@[simp] lemma IsSemiterm.func_iff {k f v : V} :
+    𝐓ⁿ (^func k f v) ↔ L.Func k f ∧ L.TermSeq k n v :=
+  ⟨by intro h
+      rcases h.case with (⟨_, _, h⟩ | ⟨x, h⟩ | ⟨k', f', v', hkf, ⟨Sv, hk, hv⟩, h⟩)
+      · simp [qqFunc, qqBvar] at h
+      · simp [qqFunc, qqFvar] at h
+      · rcases (show k = k' ∧ f = f' ∧ v = v' by simpa [qqFunc] using h) with ⟨rfl, rfl, rfl⟩
+        exact ⟨hkf, Sv, hk, hv⟩,
+   by rintro ⟨hkf, Sv, hk, hv⟩; exact Language.IsSemiterm.mk (Or.inr <| Or.inr ⟨k, f, v, hkf, ⟨Sv, hk, hv⟩, rfl⟩)⟩
+
+lemma IsSemiterm.func {k f v : V} (hkf : L.Func k f) (hv : L.TermSeq k n v) :
+    𝐓ⁿ (^func k f v) := IsSemiterm.func_iff.mpr ⟨hkf, hv⟩
+
+lemma IsSemiterm.induction (Γ) {P : V → Prop} (hP : (Γ, 1)-Predicate P)
+    (hbvar : ∀ z < n, P (^#z)) (hfvar : ∀ x, P (^&x))
+    (hfunc : ∀ k f v, L.Func k f → L.TermSeq k n v → (∀ i u, ⟪i, u⟫ ∈ v → P u) → P (^func k f v)) :
+    ∀ t, 𝐓ⁿ t → P t :=
+  (construction L).induction (v := ![n]) hP (by
+    rintro C hC x (⟨z, hz, rfl⟩ | ⟨x, rfl⟩ | ⟨k, f, v, hkf, Sv, hk, h, rfl⟩)
+    · exact hbvar z hz
+    · exact hfvar x
+    · exact hfunc k f v hkf ⟨Sv, hk, fun i u hi ↦ hC u (h i u hi) |>.1⟩ (fun i u hi ↦ hC u (h i u hi) |>.2))
+
+end term
+
+section termSubst
+
 namespace FormalizedTermSubst
 
 variable (L)
 
-def Phi (n m w : M) (C : Set M) (p : M) : Prop :=
+def Phi (n m w : V) (C : Set V) (p : V) : Prop :=
   L.IsSemiterm n (π₁ p) ∧ L.IsSemiterm m (π₂ p) ∧
   ( (∃ z < n, π₁ p = ^#z ∧ ⟪z, π₂ p⟫ ∈ w) ∨
     (∃ x, π₁ p = ^&x ∧ π₂ p = ^&x) ∨
     (∃ k f v v', π₁ p = ^func k f v ∧ π₂ p = ^func k f v' ∧ ∀ i u u', ⟪i, u⟫ ∈ v → ⟪i, u'⟫ ∈ v' → ⟪u, u'⟫ ∈ C) )
 
-private lemma phi_iff (n m w C p : M) :
+private lemma phi_iff (n m w C p : V) :
     Phi L n m w {x | x ∈ C} p ↔
     ∃ t₁ ≤ p, ∃ t₂ ≤ p, p = ⟪t₁, t₂⟫ ∧ L.IsSemiterm n t₁ ∧ L.IsSemiterm m t₂ ∧
     ( (∃ z < n, t₁ = ^#z ∧ ⟪z, t₂⟫ ∈ w) ∨
@@ -310,7 +305,7 @@ def formula (pL : LDef) : Fixpoint.Blueprint 3 := ⟨.mkDelta
       !formulaAux t₁ t₂ p C n m w”
     (by simp [formulaAux]))⟩
 
-def construction : Fixpoint.Construction M (formula pL) where
+def construction : Fixpoint.Construction V (formula pL) where
   Φ := fun v ↦ Phi L (v 0) (v 1) (v 2)
   defined := ⟨fun v ↦
     by simp [formula, HSemiformula.val_sigma, eval_isSemitermDef L, (isSemiterm_defined L).proper.iff'],
@@ -321,7 +316,7 @@ def construction : Fixpoint.Construction M (formula pL) where
     · exact ⟨ht₁, ht₂, Or.inr <| Or.inl h⟩
     · exact ⟨ht₁, ht₂, Or.inr <| Or.inr ⟨k, f, v, v', h₁, h₂, fun i u u' hi hi' ↦ hC (h i u u' hi hi')⟩⟩
 
-instance : (construction L).StrongFinite M where
+instance : (construction L).StrongFinite V where
   strong_finite := by
     rintro C v p ⟨ht₁, ht₂, (h | h | ⟨k, f, v, v', h₁, h₂, h⟩)⟩
     · exact ⟨ht₁, ht₂, Or.inl h⟩
@@ -330,7 +325,7 @@ instance : (construction L).StrongFinite M where
       have : ⟪u, u'⟫ < ⟪π₁ p, π₂ p⟫ := pair_lt_pair (by simpa [h₁] using lt_qqFunc_of_mem hi) (by simpa [h₂] using lt_qqFunc_of_mem hi')
       simpa using this⟩⟩⟩
 
-def Subst (n m w : M) : M → Prop := (construction L).Fixpoint ![n, m, w]
+def Subst (n m w : V) : V → Prop := (construction L).Fixpoint ![n, m, w]
 
 def _root_.LO.FirstOrder.Arith.LDef.substDef (pL : LDef) : 𝚫₁-Semisentence 4 :=
   (formula pL).fixpointDefΔ₁.rew <| Rew.substs ![#3, #0, #1, #2]
@@ -340,7 +335,7 @@ lemma subst_defined : 𝚫₁-Relation₄ (Subst L) via pL.substDef :=
    by intro v; simp [LDef.substDef, (construction L).eval_fixpointDefΔ₁, Subst]⟩
 
 @[simp] lemma eval_substDef (v) :
-    Semiformula.Evalbm M v pL.substDef.val ↔ Subst L (v 0) (v 1) (v 2) (v 3) := (subst_defined L).df.iff v
+    Semiformula.Evalbm V v pL.substDef.val ↔ Subst L (v 0) (v 1) (v 2) (v 3) := (subst_defined L).df.iff v
 
 instance subst_definable : 𝚫₁-Relation₄ (Subst L) := Defined.to_definable _ (subst_defined L)
 
@@ -349,7 +344,7 @@ instance subst_definable : 𝚫₁-Relation₄ (Subst L) := Defined.to_definable
 
 variable {L}
 
-lemma Subst.case_iff {n m w p : M} :
+lemma Subst.case_iff {n m w p : V} :
     Subst L n m w p ↔
     L.IsSemiterm n (π₁ p) ∧ L.IsSemiterm m (π₂ p) ∧
     ( (∃ z < n, π₁ p = ^#z ∧ ⟪z, π₂ p⟫ ∈ w) ∨
@@ -363,10 +358,10 @@ lemma Subst.semiterm₁ {n m w t t'} (h : Subst L n m w ⟪t, t'⟫) : L.IsSemit
 
 lemma Subst.semiterm₂ {n m w t t'} (h : Subst L n m w ⟪t, t'⟫) : L.IsSemiterm m t' := by simpa using h.case.2.1
 
-lemma Subst.bvar {n m w z u : M} (hz : z < n) (hu : L.IsSemiterm m u) (h : ⟪z, u⟫ ∈ w) :
+lemma Subst.bvar {n m w z u : V} (hz : z < n) (hu : L.IsSemiterm m u) (h : ⟪z, u⟫ ∈ w) :
     Subst L n m w ⟪^#z, u⟫ := Subst.mk ⟨by simp [hz], by simpa using hu, Or.inl ⟨z, hz, by simpa using h⟩⟩
 
-lemma Subst.bvar_iff {n m w z u : M} :
+lemma Subst.bvar_iff {n m w z u : V} :
     Subst L n m w ⟪^#z, u⟫ ↔ z < n ∧ L.IsSemiterm m u ∧ ⟪z, u⟫ ∈ w :=
   ⟨by intro h
       rcases h.case with ⟨_, hu, (⟨z', hz', hzz', h⟩ | ⟨x, h, _⟩ | ⟨k, f, v, v', h, _⟩)⟩
@@ -375,10 +370,10 @@ lemma Subst.bvar_iff {n m w z u : M} :
       · simp [qqBvar, qqFunc] at h,
    by rintro ⟨hz, Hu, h⟩; exact Subst.bvar hz Hu h⟩
 
-@[simp] lemma Subst.fvar {n m w x : M} :
+@[simp] lemma Subst.fvar {n m w x : V} :
     Subst L n m w ⟪^&x, ^&x⟫ := Subst.mk ⟨by simp, by simp, Or.inr <| Or.inl ⟨x, by simp⟩⟩
 
-lemma Subst.fvar_iff {n m w x u : M} :
+lemma Subst.fvar_iff {n m w x u : V} :
     Subst L n m w ⟪^&x, u⟫ ↔ u = ^&x := by
   constructor
   · intro h
@@ -388,22 +383,18 @@ lemma Subst.fvar_iff {n m w x u : M} :
     · simp [qqFvar, qqFunc] at h
   · rintro rfl; simp
 
-lemma Subst.func {n m w k f v v' : M}
+lemma Subst.func {n m w k f v v' : V}
     (hkf : L.Func k f)
-    (Sv : Seq v)
-    (hk : k = lh v)
-    (hv : ∀ i u, ⟪i, u⟫ ∈ v → L.IsSemiterm n u)
-    (Sv' : Seq v')
-    (hk' : k = lh v')
-    (hv' : ∀ i u', ⟪i, u'⟫ ∈ v' → L.IsSemiterm m u')
+    (hv : L.TermSeq k n v)
+    (hv' : L.TermSeq k m v')
     (H : ∀ i u u', ⟪i, u⟫ ∈ v → ⟪i, u'⟫ ∈ v' → Subst L n m w ⟪u, u'⟫) :
     Subst L n m w ⟪^func k f v, ^func k f v'⟫ :=
   Subst.mk ⟨
-    by rw [pi₁_pair]; exact IsSemiterm.func hkf Sv hk hv,
-    by rw [pi₂_pair]; exact IsSemiterm.func hkf Sv' hk' hv',
+    by rw [pi₁_pair]; exact IsSemiterm.func hkf hv,
+    by rw [pi₂_pair]; exact IsSemiterm.func hkf hv',
     Or.inr <| Or.inr ⟨k, f, v, v', by simp, by simp, H⟩⟩
 
-lemma Subst.func' {n m w k f v u : M} (h : Subst L n m w ⟪^func k f v, u⟫) :
+lemma Subst.func' {n m w k f v u : V} (h : Subst L n m w ⟪^func k f v, u⟫) :
     ∃ v', Seq v' ∧ k = lh v' ∧ (∀ i u u', ⟪i, u⟫ ∈ v → ⟪i, u'⟫ ∈ v' → Subst L n m w ⟪u, u'⟫) ∧ u = ^func k f v' := by
   rcases h.case with ⟨_, hu, (⟨_, _, h, _⟩ | ⟨x, h, _⟩ | ⟨k', f', v', v'', h₁, h₂, hv⟩)⟩
   · simp [qqFunc, qqBvar] at h
@@ -416,7 +407,7 @@ lemma Subst.func' {n m w k f v u : M} (h : Subst L n m w ⟪^func k f v, u⟫) :
 
 variable {n m w} (TSw : L.TermSeq n m w)
 
-lemma Subst.rng_exists {t : M} (ht : L.IsSemiterm n t) : ∃ u, Subst L n m w ⟪t, u⟫ := by
+lemma Subst.rng_exists {t : V} (ht : L.IsSemiterm n t) : ∃ u, Subst L n m w ⟪t, u⟫ := by
   apply IsSemiterm.induction 𝚺 ?_ ?_ ?_ ?_ t ht
   · definability
   · intro z hz
@@ -424,27 +415,27 @@ lemma Subst.rng_exists {t : M} (ht : L.IsSemiterm n t) : ∃ u, Subst L n m w �
     rcases this with ⟨u, hu⟩
     exact ⟨u, Subst.bvar hz (TSw.prop z u hu) hu⟩
   · intro x; exact ⟨^&x, by simp⟩
-  · rintro k f v hkf Sv rfl ih
+  · rintro k f v hkf hv ih
     have : ∃ v', Seq v' ∧ lh v' = lh v ∧ ∀ i u', ⟪i, u'⟫ ∈ v' → ∀ u, ⟪i, u⟫ ∈ v → Subst L n m w ⟪u, u'⟫ := by
       have : ∀ i < lh v, ∃ u', ∀ u, ⟪i, u⟫ ∈ v → Subst L n m w ⟪u, u'⟫ := by
         intro i hi
-        have : L.IsSemiterm n (Sv.nth hi) ∧ ∃ u, Subst L n m w ⟪Sv.nth hi, u⟫ := ih i (Sv.nth hi) (by simp)
-        rcases this with ⟨_, u', hu'⟩
-        exact ⟨u', fun u hiuv  ↦ by rcases Sv.nth_uniq hi hiuv; exact hu'⟩
+        have : ∃ u, Subst L n m w ⟪hv.seq.nth hi, u⟫ := ih i (hv.seq.nth hi) (by simp)
+        rcases this with ⟨u', hu'⟩
+        exact ⟨u', fun u hiuv  ↦ by rcases hv.seq.nth_uniq hi hiuv; exact hu'⟩
       exact sigmaOne_skolem_seq
         (by have : 𝚺₁-Relation fun x y ↦ ∀ u < v, ⟪x, u⟫ ∈ v → Subst L n m w ⟪u, y⟫ := by definability
             exact this.of_iff fun w ↦ ⟨fun h u _ ↦ h u, fun h u hv ↦ h u (lt_of_mem_rng hv) hv⟩)
         this
     rcases this with ⟨v', Sv', hvv', h⟩
-    exact ⟨^func (lh v) f v',
-      Subst.func hkf Sv rfl (fun i u hi ↦ (ih i u hi).1) Sv' (Eq.symm hvv')
+    exact ⟨^func k f v',
+      Subst.func hkf hv ⟨Sv', by simp [hvv', hv.lh],
         (fun i u' hi ↦ by
           have : i < lh v := by simpa [hvv'] using Sv'.lt_lh_of_mem hi
-          exact h i u' hi (Sv.nth this) (by simp) |>.semiterm₂)
+          exact h i u' hi (hv.seq.nth this) (by simp) |>.semiterm₂)⟩
         (fun i u u' hi hi' ↦ h i u' hi' u hi)⟩
 
 lemma Subst.rng_unique
-    {t u₁ u₂ : M} : Subst L n m w ⟪t, u₁⟫ → Subst L n m w ⟪t, u₂⟫ → u₁ = u₂ := by
+    {t u₁ u₂ : V} : Subst L n m w ⟪t, u₁⟫ → Subst L n m w ⟪t, u₂⟫ → u₁ = u₂ := by
   revert u₁ u₂
   suffices L.IsSemiterm n t → ∀ u₁ u₂, Subst L n m w ⟪t, u₁⟫ → Subst L n m w ⟪t, u₂⟫ → u₁ = u₂
   by intro u₁ u₂ h₁ h₂; exact this h₁.semiterm₁ u₁ u₂ h₁ h₂
@@ -455,22 +446,22 @@ lemma Subst.rng_unique
     intro z _ u₁ u₂ _ _ h₁ _ _ h₂
     exact TSw.seq.isMapping.uniq h₁ h₂
   · simp [Subst.fvar_iff]
-  · intro k f v _ Sv hk ih u₁ u₂ h₁ h₂
+  · intro k f v _ hv ih u₁ u₂ h₁ h₂
     rcases Subst.func' h₁ with ⟨v₁, Sv₁, hk₁, hvv₁, rfl⟩
     rcases Subst.func' h₂ with ⟨v₂, Sv₂, hk₂, hvv₂, rfl⟩
     have : v₁ = v₂ := Sv₁.lh_ext Sv₂ (by simp [←hk₁, ←hk₂]) (by
       intro i x₁ x₂ hxv₁ hxv₂
-      have hi : i < lh v := by simpa [←hk, hk₁] using Sv₁.lt_lh_of_mem hxv₁
-      exact ih i (Sv.nth hi) (by simp) |>.2 _ _ (hvv₁ _ _ _ (Sv.nth_mem hi) hxv₁) (hvv₂ _ _ _ (Sv.nth_mem hi) hxv₂))
+      have hi : i < lh v := by simpa [←hv.lh, hk₁] using Sv₁.lt_lh_of_mem hxv₁
+      exact ih i (hv.seq.nth hi) (by simp) _ _ (hvv₁ _ _ _ (hv.seq.nth_mem hi) hxv₁) (hvv₂ _ _ _ (hv.seq.nth_mem hi) hxv₂))
     rw [this]
 
-lemma Subst.rng_exists_unique {t : M} (ht : L.IsSemiterm n t) : ∃! u, Subst L n m w ⟪t, u⟫ := by
+lemma Subst.rng_exists_unique {t : V} (ht : L.IsSemiterm n t) : ∃! u, Subst L n m w ⟪t, u⟫ := by
   rcases Subst.rng_exists TSw ht with ⟨u, hu⟩
   exact ExistsUnique.intro u hu (fun u' hu' ↦ Subst.rng_unique TSw hu' hu)
 
 variable (L)
 
-lemma Subst.rng_exists_unique_total (n m w t : M) :
+lemma Subst.rng_exists_unique_total (n m w t : V) :
     ∃! u, (L.TermSeq n m w ∧ L.IsSemiterm n t → Subst L n m w ⟪t, u⟫) ∧ (¬(L.TermSeq n m w ∧ L.IsSemiterm n t) → u = 0) := by
   by_cases h : L.TermSeq n m w ∧ L.IsSemiterm n t
   · simp [h]; exact Subst.rng_exists_unique h.1 h.2
@@ -482,41 +473,41 @@ open FormalizedTermSubst
 
 variable (L)
 
-def Language.termSubst (n m w t : M) : M := Classical.choose! (Subst.rng_exists_unique_total L n m w t)
+def Language.termSubst (n m w t : V) : V := Classical.choose! (Subst.rng_exists_unique_total L n m w t)
 
 variable {L}
 
-def Language.TermSeq.spec_of_semiterm {n m w t : M} (TSw : L.TermSeq n m w) (ht : L.IsSemiterm n t) : Subst L n m w ⟪t, L.termSubst n m w t⟫ :=
+def Language.TermSeq.spec_of_semiterm {n m w t : V} (TSw : L.TermSeq n m w) (ht : L.IsSemiterm n t) : Subst L n m w ⟪t, L.termSubst n m w t⟫ :=
   Classical.choose!_spec (Subst.rng_exists_unique_total L n m w t) |>.1 ⟨TSw, ht⟩
 
-def termSubst_spec {n m w t : M} :
+def termSubst_spec {n m w t : V} :
     ¬(L.TermSeq n m w ∧ L.IsSemiterm n t) → L.termSubst n m w t = 0 :=
   Classical.choose!_spec (Subst.rng_exists_unique_total L n m w t) |>.2
 
-variable {n m w : M} (TSw : L.TermSeq n m w)
+variable {n m w : V} (TSw : L.TermSeq n m w)
 
 lemma Language.TermSeq.termSubst_eq_of {t} (ht : L.IsSemiterm n t) (h : Subst L n m w ⟪t, u⟫) : L.termSubst n m w t = u :=
   (TSw.spec_of_semiterm ht).rng_unique TSw h
 
-lemma termSubst_bvar {z : M} (hz : z < n) (hu : ⟪z, u⟫ ∈ w) : L.termSubst n m w (^#z) = u :=
+lemma termSubst_bvar {z : V} (hz : z < n) (hu : ⟪z, u⟫ ∈ w) : L.termSubst n m w (^#z) = u :=
   TSw.termSubst_eq_of (by simp [hz]) (Subst.bvar hz (TSw.prop z u hu) hu)
 
-@[simp] lemma termSubst_fvar (x : M) : L.termSubst n m w (^&x) = ^&x :=
+@[simp] lemma termSubst_fvar (x : V) : L.termSubst n m w (^&x) = ^&x :=
   TSw.termSubst_eq_of (by simp) (by simp)
 
-lemma termSubst_func {k f v v' : M} (hfk : L.Func k f)
-    (Sv : Seq v) (hk : k = lh v) (hv : ∀ i u, ⟪i, u⟫ ∈ v → L.IsSemiterm n u)
-    (Sv' : Seq v') (hk' : k = lh v') (hv' : ∀ i u', ⟪i, u'⟫ ∈ v' → L.IsSemiterm m u')
+lemma termSubst_func {k f v v' : V} (hfk : L.Func k f)
+    (hv : L.TermSeq k n v)
+    (hv' : L.TermSeq k m v')
     (H : ∀ i u u', ⟪i, u⟫ ∈ v → ⟪i, u'⟫ ∈ v' → L.termSubst n m w u = u') : L.termSubst n m w (^func k f v) = ^func k f v' :=
-  TSw.termSubst_eq_of (IsSemiterm.func hfk Sv hk hv)
-    (Subst.func hfk Sv hk hv Sv' hk' hv' (fun i u u' hi hi' ↦ by
-      rcases H i u u' hi hi'; exact TSw.spec_of_semiterm (hv i u hi)))
+  TSw.termSubst_eq_of (IsSemiterm.func hfk hv)
+    (Subst.func hfk hv hv' (fun i u u' hi hi' ↦ by
+      rcases H i u u' hi hi'; exact TSw.spec_of_semiterm (hv.prop i u hi)))
 
 section
 
 variable (L)
 
-private lemma termSubst_graph (u n m w t : M) :
+private lemma termSubst_graph (u n m w t : V) :
     u = L.termSubst n m w t ↔
     (L.TermSeq n m w ∧ L.IsSemiterm n t → ∃ p ≤ (t + u + 1)^2, p = ⟪t, u⟫ ∧ Subst L n m w p) ∧ (¬(L.TermSeq n m w ∧ L.IsSemiterm n t) → u = 0) :=
   Iff.trans (Classical.choose!_eq_iff (Subst.rng_exists_unique_total L n m w t)) ⟨by
@@ -535,8 +526,8 @@ lemma termSubst_defined : 𝚺₁-Function₄ L.termSubst via pL.termSubstDef :=
     eval_isSemitermDef L, (termSeq_defined L).proper.iff', (isSemiterm_defined L).proper.iff', eval_substDef L, -and_imp, -not_and]
   apply iff_of_eq; congr; simp [imp_iff_not_or]; rfl
 
-@[simp] lemma termSubst_defined_iff (v : Fin 5 → M) :
-    Semiformula.Evalbm (L := ℒₒᵣ) M v pL.termSubstDef ↔ v 0 = L.termSubst (v 1) (v 2) (v 3) (v 4) := (termSubst_defined L).df.iff v
+@[simp] lemma termSubst_defined_iff (v : Fin 5 → V) :
+    Semiformula.Evalbm (L := ℒₒᵣ) V v pL.termSubstDef ↔ v 0 = L.termSubst (v 1) (v 2) (v 3) (v 4) := (termSubst_defined L).df.iff v
 
 instance termSubst_definable : 𝚺₁-Function₄ L.termSubst :=
   Defined.to_definable _ (termSubst_defined L)
@@ -551,13 +542,13 @@ namespace FormalizedTermShift
 
 variable (L)
 
-def Phi (n : M) (C : Set M) (p : M) : Prop :=
+def Phi (n : V) (C : Set V) (p : V) : Prop :=
   L.IsSemiterm n (π₁ p) ∧ L.IsSemiterm n (π₂ p) ∧
   ( (∃ z < n, π₁ p = ^#z ∧ π₂ p = ^#z) ∨
     (∃ x, π₁ p = ^&x ∧ π₂ p = ^&(x + 1)) ∨
     (∃ k f v v', π₁ p = ^func k f v ∧ π₂ p = ^func k f v' ∧ ∀ i u u', ⟪i, u⟫ ∈ v → ⟪i, u'⟫ ∈ v' → ⟪u, u'⟫ ∈ C) )
 
-private lemma phi_iff (n C p : M) :
+private lemma phi_iff (n C p : V) :
     Phi L n {x | x ∈ C} p ↔
     ∃ t₁ ≤ p, ∃ t₂ ≤ p, p = ⟪t₁, t₂⟫ ∧ L.IsSemiterm n t₁ ∧ L.IsSemiterm n t₂ ∧
     ( (∃ z < n, t₁ = ^#z ∧ t₂ = ^#z) ∨
@@ -600,7 +591,7 @@ def formula (pL : LDef) : Fixpoint.Blueprint 1 := ⟨.mkDelta
       !formulaAux t₁ t₂ p C n”
     (by simp [formulaAux]))⟩
 
-def construction : Fixpoint.Construction M (formula pL) where
+def construction : Fixpoint.Construction V (formula pL) where
   Φ := fun v ↦ Phi L (v 0)
   defined := ⟨fun v ↦
     by simp [formula, HSemiformula.val_sigma, eval_isSemitermDef L, (isSemiterm_defined L).proper.iff'],
@@ -611,7 +602,7 @@ def construction : Fixpoint.Construction M (formula pL) where
     · exact ⟨ht₁, ht₂, Or.inr <| Or.inl h⟩
     · exact ⟨ht₁, ht₂, Or.inr <| Or.inr ⟨k, f, v, v', h₁, h₂, fun i u u' hi hi' ↦ hC (h i u u' hi hi')⟩⟩
 
-instance : (construction L).StrongFinite M where
+instance : (construction L).StrongFinite V where
   strong_finite := by
     rintro C v p ⟨ht₁, ht₂, (h | h | ⟨k, f, v, v', h₁, h₂, h⟩)⟩
     · exact ⟨ht₁, ht₂, Or.inl h⟩
@@ -620,7 +611,7 @@ instance : (construction L).StrongFinite M where
       have : ⟪u, u'⟫ < ⟪π₁ p, π₂ p⟫ := pair_lt_pair (by simpa [h₁] using lt_qqFunc_of_mem hi) (by simpa [h₂] using lt_qqFunc_of_mem hi')
       simpa using this⟩⟩⟩
 
-def Shift (n : M) : M → Prop := (construction L).Fixpoint ![n]
+def Shift (n : V) : V → Prop := (construction L).Fixpoint ![n]
 
 def shiftDef (pL : LDef) : 𝚫₁-Semisentence 2 := (formula pL).fixpointDefΔ₁.rew <| Rew.substs ![#1, #0]
 
@@ -629,7 +620,7 @@ lemma shift_defined : 𝚫₁-Relation (Shift L) via (shiftDef pL) :=
    by intro v; simp [shiftDef, (construction L).eval_fixpointDefΔ₁, Shift]⟩
 
 @[simp] lemma eval_shiftDef (v) :
-    Semiformula.Evalbm M v (shiftDef pL).val ↔ Shift L (v 0) (v 1) := (shift_defined L).df.iff v
+    Semiformula.Evalbm V v (shiftDef pL).val ↔ Shift L (v 0) (v 1) := (shift_defined L).df.iff v
 
 instance shift_definable : 𝚫₁-Relation (Shift L) := Defined.to_definable _ (shift_defined L)
 
@@ -638,7 +629,7 @@ instance shift_definable : 𝚫₁-Relation (Shift L) := Defined.to_definable _ 
 
 variable {L}
 
-lemma Shift.case_iff {n p : M} :
+lemma Shift.case_iff {n p : V} :
     Shift L n p ↔
     L.IsSemiterm n (π₁ p) ∧ L.IsSemiterm n (π₂ p) ∧
     ( (∃ z < n, π₁ p = ^#z ∧ π₂ p = ^#z) ∨
@@ -652,10 +643,10 @@ lemma Shift.semiterm₁ {n t t'} (h : Shift L n ⟪t, t'⟫) : L.IsSemiterm n t 
 
 lemma Shift.semiterm₂ {n t t'} (h : Shift L n ⟪t, t'⟫) : L.IsSemiterm n t' := by simpa using h.case.2.1
 
-@[simp] lemma Shift.bvar {n z : M} (hz : z < n) :
+@[simp] lemma Shift.bvar {n z : V} (hz : z < n) :
     Shift L n ⟪^#z, ^#z⟫ := Shift.mk ⟨by simp [hz], by simp [hz]⟩
 
-lemma Shift.bvar_iff {n z u : M} :
+lemma Shift.bvar_iff {n z u : V} :
     Shift L n ⟪^#z, u⟫ ↔ z < n ∧ u = ^#z :=
   ⟨by intro h
       rcases h.case with ⟨_, _, (⟨z', hz', hzz', h⟩ | ⟨x, h, _⟩ | ⟨k, f, v, v', h, _⟩)⟩
@@ -664,10 +655,10 @@ lemma Shift.bvar_iff {n z u : M} :
       · simp [qqBvar, qqFunc] at h,
    by rintro ⟨hz, Hu, h⟩; exact Shift.bvar hz⟩
 
-@[simp] lemma Shift.fvar {n : M} (x : M):
+@[simp] lemma Shift.fvar {n : V} (x : V):
     Shift L n ⟪^&x, ^&(x + 1)⟫ := Shift.mk ⟨by simp, by simp⟩
 
-lemma Shift.fvar_iff {n x u : M} :
+lemma Shift.fvar_iff {n x u : V} :
     Shift L n ⟪^&x, u⟫ ↔ u = ^&(x + 1) :=
   ⟨by intro h
       rcases h.case with ⟨_, _, (⟨_, _, h, _⟩ | ⟨x', hx', h⟩ | ⟨_, _, _, _, h, _, _⟩)⟩
@@ -676,22 +667,18 @@ lemma Shift.fvar_iff {n x u : M} :
       · simp [qqFvar, qqFunc] at h,
    by rintro ⟨hz, Hu, h⟩; exact Shift.fvar x⟩
 
-lemma Shift.func {n k f v v' : M}
+lemma Shift.func {n k f v v' : V}
     (hkf : L.Func k f)
-    (Sv : Seq v)
-    (hk : k = lh v)
-    (hv : ∀ i u, ⟪i, u⟫ ∈ v → L.IsSemiterm n u)
-    (Sv' : Seq v')
-    (hk' : k = lh v')
-    (hv' : ∀ i u', ⟪i, u'⟫ ∈ v' → L.IsSemiterm n u')
+    (hv : L.TermSeq k n v)
+    (hv' : L.TermSeq k n v')
     (H : ∀ i u u', ⟪i, u⟫ ∈ v → ⟪i, u'⟫ ∈ v' → Shift L n ⟪u, u'⟫) :
     Shift L n ⟪^func k f v, ^func k f v'⟫ :=
   Shift.mk ⟨
-    by rw [pi₁_pair]; exact IsSemiterm.func hkf Sv hk hv,
-    by rw [pi₂_pair]; exact IsSemiterm.func hkf Sv' hk' hv',
+    by rw [pi₁_pair]; exact IsSemiterm.func hkf hv,
+    by rw [pi₂_pair]; exact IsSemiterm.func hkf hv',
     Or.inr <| Or.inr ⟨k, f, v, v', by simp, by simp, H⟩⟩
 
-lemma Shift.func' {n k f v u : M} (h : Shift L n ⟪^func k f v, u⟫) :
+lemma Shift.func' {n k f v u : V} (h : Shift L n ⟪^func k f v, u⟫) :
     ∃ v', Seq v' ∧ k = lh v' ∧ (∀ i u u', ⟪i, u⟫ ∈ v → ⟪i, u'⟫ ∈ v' → Shift L n ⟪u, u'⟫) ∧ u = ^func k f v' := by
   rcases h.case with ⟨_, hu, (⟨_, _, h, _⟩ | ⟨x, h, _⟩ | ⟨k', f', v', v'', h₁, h₂, hv⟩)⟩
   · simp [qqFunc, qqBvar] at h
@@ -702,34 +689,34 @@ lemma Shift.func' {n k f v u : M} (h : Shift L n ⟪^func k f v, u⟫) :
     rcases this with ⟨_, Sv'', hk'', _⟩
     exact ⟨v'', Sv'', hk'', hv, rfl⟩
 
-variable {n : M}
+variable {n : V}
 
-lemma Shift.rng_exists {t : M} (ht : L.IsSemiterm n t) : ∃ u, Shift L n ⟪t, u⟫ := by
+lemma Shift.rng_exists {t : V} (ht : L.IsSemiterm n t) : ∃ u, Shift L n ⟪t, u⟫ := by
   apply IsSemiterm.induction 𝚺 ?_ ?_ ?_ ?_ t ht
   · definability
   · intro z hz; exact ⟨^#z, Shift.bvar hz⟩
   · intro x; exact ⟨^&(x + 1), by simp⟩
-  · rintro k f v hkf Sv rfl ih
+  · rintro k f v hkf hv ih
     have : ∃ v', Seq v' ∧ lh v' = lh v ∧ ∀ i u', ⟪i, u'⟫ ∈ v' → ∀ u, ⟪i, u⟫ ∈ v → Shift L n ⟪u, u'⟫ := by
       have : ∀ i < lh v, ∃ u', ∀ u, ⟪i, u⟫ ∈ v → Shift L n ⟪u, u'⟫ := by
         intro i hi
-        have : L.IsSemiterm n (Sv.nth hi) ∧ ∃ u, Shift L n ⟪Sv.nth hi, u⟫ := ih i (Sv.nth hi) (by simp)
-        rcases this with ⟨_, u', hu'⟩
-        exact ⟨u', fun u hiuv  ↦ by rcases Sv.nth_uniq hi hiuv; exact hu'⟩
+        have : ∃ u, Shift L n ⟪hv.seq.nth hi, u⟫ := ih i (hv.seq.nth hi) (by simp)
+        rcases this with ⟨u', hu'⟩
+        exact ⟨u', fun u hiuv  ↦ by rcases hv.seq.nth_uniq hi hiuv; exact hu'⟩
       exact sigmaOne_skolem_seq
         (by have : 𝚺₁-Relation fun x y ↦ ∀ u < v, ⟪x, u⟫ ∈ v → Shift L n ⟪u, y⟫ := by definability
             exact this.of_iff fun w ↦ ⟨fun h u _ ↦ h u, fun h u hv ↦ h u (lt_of_mem_rng hv) hv⟩)
         this
     rcases this with ⟨v', Sv', hvv', h⟩
-    exact ⟨^func (lh v) f v',
-      Shift.func hkf Sv rfl (fun i u hi ↦ (ih i u hi).1) Sv' (Eq.symm hvv')
+    exact ⟨^func k f v',
+      Shift.func hkf hv ⟨Sv', by simp [hvv', hv.lh],
         (fun i u' hi ↦ by
           have : i < lh v := by simpa [hvv'] using Sv'.lt_lh_of_mem hi
-          exact h i u' hi (Sv.nth this) (by simp) |>.semiterm₂)
+          exact h i u' hi (hv.seq.nth this) (by simp) |>.semiterm₂)⟩
         (fun i u u' hi hi' ↦ h i u' hi' u hi)⟩
 
 lemma Shift.rng_unique
-    {t u₁ u₂ : M} : Shift L n ⟪t, u₁⟫ → Shift L n ⟪t, u₂⟫ → u₁ = u₂ := by
+    {t u₁ u₂ : V} : Shift L n ⟪t, u₁⟫ → Shift L n ⟪t, u₂⟫ → u₁ = u₂ := by
   revert u₁ u₂
   suffices L.IsSemiterm n t → ∀ u₁ u₂, Shift L n ⟪t, u₁⟫ → Shift L n ⟪t, u₂⟫ → u₁ = u₂
   by intro u₁ u₂ h₁ h₂; exact this h₁.semiterm₁ u₁ u₂ h₁ h₂
@@ -739,22 +726,22 @@ lemma Shift.rng_unique
   · simp only [bvar_iff, and_imp]
     rintro z _ u₁ u₂ _ rfl _ rfl; rfl
   · simp [Shift.fvar_iff]
-  · intro k f v _ Sv hk ih u₁ u₂ h₁ h₂
+  · intro k f v _ hv ih u₁ u₂ h₁ h₂
     rcases Shift.func' h₁ with ⟨v₁, Sv₁, hk₁, hvv₁, rfl⟩
     rcases Shift.func' h₂ with ⟨v₂, Sv₂, hk₂, hvv₂, rfl⟩
     have : v₁ = v₂ := Sv₁.lh_ext Sv₂ (by simp [←hk₁, ←hk₂]) (by
       intro i x₁ x₂ hxv₁ hxv₂
-      have hi : i < lh v := by simpa [←hk, hk₁] using Sv₁.lt_lh_of_mem hxv₁
-      exact ih i (Sv.nth hi) (by simp) |>.2 _ _ (hvv₁ _ _ _ (Sv.nth_mem hi) hxv₁) (hvv₂ _ _ _ (Sv.nth_mem hi) hxv₂))
+      have hi : i < lh v := by simpa [←hv.lh, hk₁] using Sv₁.lt_lh_of_mem hxv₁
+      exact ih i (hv.seq.nth hi) (by simp) _ _ (hvv₁ _ _ _ (hv.seq.nth_mem hi) hxv₁) (hvv₂ _ _ _ (hv.seq.nth_mem hi) hxv₂))
     rw [this]
 
-lemma Shift.rng_exists_unique {t : M} (ht : L.IsSemiterm n t) : ∃! u, Shift L n ⟪t, u⟫ := by
+lemma Shift.rng_exists_unique {t : V} (ht : L.IsSemiterm n t) : ∃! u, Shift L n ⟪t, u⟫ := by
   rcases Shift.rng_exists ht with ⟨u, hu⟩
   exact ExistsUnique.intro u hu (fun u' hu' ↦ Shift.rng_unique hu' hu)
 
 variable (L)
 
-lemma Shift.rng_exists_unique_total (n t : M) :
+lemma Shift.rng_exists_unique_total (n t : V) :
     ∃! u, (L.IsSemiterm n t → Shift L n ⟪t, u⟫) ∧ (¬L.IsSemiterm n t → u = 0) := by
   by_cases h : L.IsSemiterm n t
   · simp [h]; exact Shift.rng_exists_unique h
@@ -766,40 +753,40 @@ open FormalizedTermShift
 
 variable (L)
 
-def Language.termShift (n t : M) : M := Classical.choose! (Shift.rng_exists_unique_total L n t)
+def Language.termShift (n t : V) : V := Classical.choose! (Shift.rng_exists_unique_total L n t)
 
 variable {L}
 
-lemma Language.IsSemiterm.termShift_spec {n t : M} (ht : L.IsSemiterm n t) : Shift L n ⟪t, L.termShift n t⟫ :=
+lemma Language.IsSemiterm.termShift_spec {n t : V} (ht : L.IsSemiterm n t) : Shift L n ⟪t, L.termShift n t⟫ :=
   Classical.choose!_spec (Shift.rng_exists_unique_total L n t) |>.1 ht
 
-lemma termShift_spec_of_not_termShift {n t : M} :
+lemma termShift_spec_of_not_termShift {n t : V} :
     ¬L.IsSemiterm n t → L.termShift n t = 0 :=
   Classical.choose!_spec (Shift.rng_exists_unique_total L n t) |>.2
 
 lemma Language.IsSemiterm.termShift_eq_of {n t} (ht : L.IsSemiterm n t) (h : Shift L n ⟪t, u⟫) : L.termShift n t = u :=
   ht.termShift_spec.rng_unique h
 
-lemma termShift_bvar {z : M} (hz : z < n) : L.termShift n (^#z) = ^#z :=
+lemma termShift_bvar {z : V} (hz : z < n) : L.termShift n (^#z) = ^#z :=
   Language.IsSemiterm.termShift_eq_of (by simp [hz]) (Shift.bvar hz)
 
-@[simp] lemma termShift_fvar (x : M) : L.termShift n (^&x) = ^&(x + 1) :=
+@[simp] lemma termShift_fvar (x : V) : L.termShift n (^&x) = ^&(x + 1) :=
   Language.IsSemiterm.termShift_eq_of (by simp) (Shift.fvar x)
 
-lemma termShift_func {k f v v' : M} (hfk : L.Func k f)
-    (Sv : Seq v) (hk : k = lh v) (hv : ∀ i u, ⟪i, u⟫ ∈ v → L.IsSemiterm n u)
-    (Sv' : Seq v') (hk' : k = lh v') (hv' : ∀ i u', ⟪i, u'⟫ ∈ v' → L.IsSemiterm n u')
+lemma termShift_func {k f v v' : V} (hfk : L.Func k f)
+    (hv : L.TermSeq k n v)
+    (hv' : L.TermSeq k n v')
     (H : ∀ i u u', ⟪i, u⟫ ∈ v → ⟪i, u'⟫ ∈ v' → L.termShift n u = u') : L.termShift n (^func k f v) = ^func k f v' :=
-  Language.IsSemiterm.termShift_eq_of (IsSemiterm.func hfk Sv hk hv)
-    (Shift.func hfk Sv hk hv Sv' hk' hv' (fun i u u' hi hi' ↦ by
+  Language.IsSemiterm.termShift_eq_of (IsSemiterm.func hfk hv)
+    (Shift.func hfk hv hv' (fun i u u' hi hi' ↦ by
       rcases H i u u' hi hi'
-      exact Language.IsSemiterm.termShift_spec (hv i u hi)))
+      exact Language.IsSemiterm.termShift_spec (hv.prop i u hi)))
 
 section
 
 variable (L)
 
-private lemma termShift_graph (u n t : M) :
+private lemma termShift_graph (u n t : V) :
     u = L.termShift n t ↔
     (L.IsSemiterm n t → ∃ p ≤ (t + u + 1)^2, p = ⟪t, u⟫ ∧ Shift L n p) ∧ (¬L.IsSemiterm n t → u = 0) :=
   Iff.trans (Classical.choose!_eq_iff (Shift.rng_exists_unique_total L n t)) ⟨by
@@ -816,8 +803,8 @@ lemma termShift_defined : 𝚺₁-Function₂ L.termShift via pL.termShiftDef :=
   simp [LDef.termShiftDef, termShift_graph, HSemiformula.val_sigma, eval_termSeq L,
     eval_isSemitermDef L, (termSeq_defined L).proper.iff', (isSemiterm_defined L).proper.iff', eval_shiftDef L, -and_imp, -not_and]
 
-@[simp] lemma termShift_defined_iff (v : Fin 3 → M) :
-    Semiformula.Evalbm (L := ℒₒᵣ) M v pL.termShiftDef ↔ v 0 = L.termShift (v 1) (v 2) := (termShift_defined L).df.iff v
+@[simp] lemma termShift_defined_iff (v : Fin 3 → V) :
+    Semiformula.Evalbm (L := ℒₒᵣ) V v pL.termShiftDef ↔ v 0 = L.termShift (v 1) (v 2) := (termShift_defined L).df.iff v
 
 instance termShift_definable : 𝚺₁-Function₂ L.termShift :=
   Defined.to_definable _ (termShift_defined L)
